\begin{enumerate}[label=\ilabel]
    \item 
        If $f$ of degree $d$ and $g$ is of degree $e$, then we have:
        \begin{gather*}
            f^* = x_n^d f(\frac{x_1}{x_n}, \frac{x_2}{x_n}, \dots, \frac{x_{n - 1}}{x_n}) \\
            g^* = x_n^e g(\frac{x_1}{x_n}, \frac{x_2}{x_n}, \dots, \frac{x_{n - 1}}{x_n})
        \end{gather*}
        And since $fg$ is of degree $e + d$, then we have:
        \begin{gather*}
            (fg)^* = x_n^{d + e} fg(\frac{x_1}{x_n}, \frac{x_2}{x_n}, \dots, \frac{x_{n - 1}}{x_n})
        \end{gather*}
        Now it is easy to see that $(fg)^* = f^* g^*$. \\
        As for $F_*$ and $G_*$ we have:
        \begin{gather*}
            F_* = F(x_1, x_2, \dots, x_{n - 1}, 1) \\
            G_* = G(x_1, x_2, \dots, x_{n - 1}, 1) \\
            (FG)* = FG(x_1, x_2, \dots, x_{n - 1}, 1)
        \end{gather*}
        Thus we have: $(FG)_* = F_* G_*$. 
    \item 
        Suppose $f$ is of degree $d$:
        \begin{gather*}
            (f^*)_* = (x_{n + 1}^d f(\frac{x_1}{x_{n + 1}}, \frac{x_2}{x_{n+ 1}}, \dots, \frac{x_{n}}{x_{n + 1}}))_*
        \end{gather*}
        Now if we let $g(x_1, x_2, \dots, x_n, x_{n + 1}) = x_{n + 1}^d f(\frac{x_1}{x_{n + 1}}, \frac{x_2}{x_{n+ 1}}, \dots, \frac{x_{n}}{x_{n + 1}})$, Then we have:
        \begin{gather*}
            (f^*)_* = g_* = g(x_1, x_2, \dots, x_n, 1) = 1^d f(x_1, \dots, x_n) = f
        \end{gather*}
        Also:
        \begin{gather*}
            x_{n + 1}^r (F_*)^* = x_{n + 1}^r (F(x_1, x_2, \dots, x_n, 1))^* = x_{n + 1}^r (x_{n + 1}^s F(\frac{x_1}{x_{n + 1}}, \dots, \frac{x_n}{x_{n + 1}}, 1))
        \end{gather*}
        Where $s$ is the degree of $F(x_1, x_2, \dots, x_n, 1)$. Now each term of $F$ is of the form $k x_1^{r_1} x_2^{r_2} \dots x_n^{r_n} x_{n + 1}^{r_{n + 1}}$, for some $k \in K$, Which in $x_{n + 1}^r(F_*)^*$ is transformed to:
        \begin{gather*}
            x_{n + 1}^{r + s} \frac{x_1^{r_1} \dots x_n^{r_n}}{x_{n + 1}^{r_1 + \dots + r_n}} = x_1^{r_1} x_2^{r_2} \dots x_n^{r_n} x_{n + 1}^{r + s - r_1 - r_2 - \dots - r_n}
        \end{gather*}
        Now since $F$ is homogeneous, then there is some fixed $d$ such that $r_1 + \dots + r_n + r_{n + 1} = d$. Therefore the term with the biggest degree in $F_*$ is the term with the least $r_{n + 1}$, which is $r$. This shows us that $d = s + r$. Therefore $r + s - r_1 - r_2 - \dots - r_n = r_{n + 1}$. Therefore this term is the same in both forms, and since this was an arbitrary term, then we can conclude that $x_{n + 1}^{r} (F_*)^* = F$.
    \item 
        If we have both $F, G \in K[x_1, x_2, \dots, x_n]$, then we have:
        \begin{gather*}
            \begin{split}
                (F + G)_* & = (F + G)(x_1, x_2, \dots, x_{n - 1}, 1) \\
                & = F(x_1, x_2, \dots, x_{n - 1}, 1) + G(x_1, x_2, \dots, x_{n - 1}, 1)\\
                & = F_* + G_*
            \end{split}
        \end{gather*}
        And if $f$ is of degree $d$ and $g$ is of degree $e$, and without loss of generality suppose that $d \le e$, then we have:
        \begin{gather*}
            \begin{split}
                (f + g)^* & = x_n^e (f + g)(\frac{x_1}{x_n}, \frac{x_2}{x_n}, \dots, \frac{x_{n - 1}}{x_n}) \\
                & = x_n^e f(\frac{x_1}{x_n}, \frac{x_2}{x_n}, \dots, \frac{x_{n - 1}}{x_n}) + x_n^e g(\frac{x_1}{x_n}, \frac{x_2}{x_n}, \dots, \frac{x_{n - 1}}{x_n}) \\
                & = x_n^{e - d} f^* + g^*
            \end{split}
        \end{gather*}
\end{enumerate}