\begin{enumerate}[label=\ilabel]
    \item 
        First we find the equation of the line connecting $P_1$ and $P_2$:
        \begin{gather*}
            \lambda = \frac{v_2 - v_1}{u_2 - u_1} \hspace{1cm}
            v = \lambda u + k \hspace{.3cm} \text{ where } \hspace{.3cm} k = v_1 - \lambda u_1 = v_2 - \lambda u_2 
        \end{gather*}
        Now if we substitute $u$ and $v$ from the line we get the intersections:
        \begin{gather*}
            u^3 + v^3 = u^3 + (\lambda u + k)^3 = \alpha \\
            (\lambda^3 + 1) u^3 + 3k\lambda^2 u^2 + 3k^2 \lambda u + k^3 = \alpha
        \end{gather*}
        But we know two of these roots are $u_1$ and $u_2$, so we want to find $u_3$. Note that $u_1 + u_2 + u_3 = - 3k\lambda^2 / \lambda^3 + 1$:
        \begin{gather*}
            u_3 = -\frac{3k\lambda^2}{\lambda^3 + 1} - u_1 - u_2
        \end{gather*}
        And $v_3 = \lambda u_3 + k$. This gives us the point $P_1 * P_2$. Now we have to find the intersection of the line passing through $P_1 * P_2$ and $\mathcal{O}$ with the curve. A projective line has the form $l = x + by + cz = 0$. If substitute the value for two points we have:
        \begin{gather*}
            1 - b = 0 \implies b = 1 \\
            u_3 + v_3 + c = 0
        \end{gather*}
        Therefore the line looks like this: $l = x + y - (u_3 + v_3) z = 0$. Now if we substitute this into the curve equation:
        \begin{gather*}
            U^3 + V^3 = \alpha W^3 = \alpha (\frac{U + V}{u_3 + v_3})^3
        \end{gather*}
\end{enumerate}