\begin{enumerate}[label=]
    \item 
        First we define a recursive function that returns the remainder of $m/n$.
        We use functions that are defined in problem 4.\\
        Put $f(x) = 0$ and $g(x, y, z) = \chi_{(z + 1)<x} \times (z + 1)$.
        \begin{gather*}
            h(m, 0) = f(m) \\
            h(m, n + 1) = g(m, n, d(m, n)) = \chi_{h(m, n) + 1 < m} \times (h(m, n) + 1)
        \end{gather*}
        Where $\chi_D$ is the funciton for predicate $D$.
        Now we use this function to compute $d$.
        \begin{gather*}
            d(m, n) = 1 - sg(h(m, n))
        \end{gather*}
\end{enumerate}