\begin{enumerate}[label=]
    \item 
        Suppose $(x, m) = 1$. Therefore $(m - x, m) = 1$. And for $m \ne 2$ we know that $x \ne m - x$. Otherwise we would have:
        \begin{gather*}
            x = m - x \implies 2x = m \implies x = \frac{m}{2} \implies x \mid m \implies (x, m) \ne 1
        \end{gather*}
        Which gives us the contradiction. Therefore for any $m \ne 2$ we can pair all the numbers in $\{c_1, \dots, c_{\phi(m)}\}$. And sum of all pairs are $m$ since $x + m - x = m$. Therefore $S \ezmod m 0$. For $m = 2$ we have $S = 1$. This concludes the answer.
\end{enumerate}