\begin{enumerate}[label=]
    \item 
        We can write $x$ as:
        \begin{gather*}
            x \overset{2 }{\equiv} 1 \implies x = 2k + 1 , k \in \mathbb Z\\
            x \overset{3}{\equiv} 1 \implies 2k + 1 \overset{3 }{\equiv } 1 \implies 2k \overset{3 }{\equiv } 0 \implies k = 3t, t \in \mathbb Z \\
            x = 2k + 1 = 2(3t) + 1 = 6t + 1 \\
            x \overset{7 }{\equiv } 2 \implies 6t + 1 \overset{7}{\equiv } 2 \implies 6t \overset{7 }{\equiv} 1 \implies 36t \overset{7 }{\equiv } 6 \\
            \implies t \overset{7 }{\equiv} 6 \implies t = 7s + 6 , s \in \mathbb Z\\
            x = 6t + 1 = 6(7s + 6) + 1 = 42s + 37, s \in \mathbb Z \\
            \implies x = 42s + 37 , s \in \mathbb Z
        \end{gather*}
\end{enumerate}