\begin{enumerate}[label=]
    \item
        First we have to find the $\overline{1, 3}$ part.
        \begin{gather*}
            x = 1 + \frac{1}{3 + \frac{1}{x}} \implies x = 1 + \frac{x}{3x + 1} \\
            \implies x = \frac{4x + 1}{3x + 1} \implies 3x^2 - 3x - 1 = 0 \\
            \implies x = \frac{3 \pm \sqrt{9 + 12}}{6}
        \end{gather*}
        And since $x > 0$ then we have $x = \frac{3 + \sqrt{21}}{6}$. Now we can find the value of the fraction:
        \begin{gather*}
            \alpha = 1 + \frac{1}{5 + \frac{1}{2 + \frac{1}{3 + \frac{1}{x}}}} = 1 + \frac{1}{5 + \frac{1}{2 + \frac{x}{3x + 1}}} = 1 + \frac{1}{5 + \frac{3x + 1}{7x + 2}} = 1 + \frac{7x + 2}{38x + 11} = \frac{45x + 13}{38x + 11}
        \end{gather*}
        And if we let $x = \frac{3 + \sqrt{21}}{6}$:
        \begin{gather*}
            \alpha = \frac{45(\frac{3 + \sqrt{21}}{6}) + 13}{38(\frac{3 + \sqrt{21}}{6}) + 11} = \frac{2430 + 6\sqrt{21}}{2074}
        \end{gather*}
\end{enumerate}
