\begin{enumerate}[label=]
    \item 
        Note that $d < \sqrt{d^2 + 1} < d+1$:
        \begin{gather*}
            \begin{split}
                \sqrt{d^2 + 1} = d + \sqrt{d^2 + 1} - d   &= d + \frac{d^2 + 1 - d^2}{\sqrt{d^2 + 1} + d} = d + \frac{1}{\sqrt{d^2 + 1} + d} \\
                &= d + \frac{1}{2d + \sqrt{d^2 + 1} - d}
            \end{split}
        \end{gather*}
        Thus we have:
        \begin{gather*}
            \sqrt{d^2 + 1} - d = \frac{1}{2d + (\sqrt{d^2 + 1} - d)} \implies \sqrt{d^2 + 1} - d = [\overline{2d}]
        \end{gather*}
        Therefore $\sqrt{d^2 + 1} = d +(\sqrt{d^2 + 1} - d) = [d; \overline{2d}]$.
\end{enumerate}