\begin{enumerate}[label=]
   \item 
      We know that either $\frac{p_k}{q_k} < \alpha < \frac{p_{k + 1}}{q_{k + 1}}$ or $\frac{p_{k+1}}{q_{k + 1}} < \alpha < \frac{p_k}{q_k}$. This means that $\alpha - \frac{p_k}{q_k}$ and $\frac{p_{k + 1}}{q_{k + 1}} - \alpha$ have the same sign. Suppose that both $\big|\alpha - \frac{p_k}{q_k}\big| \ge \frac{1}{2q_k^2}$ and $\big|\alpha - \frac{p_{k + 1}}{q_{k + 1}}\big| \ge \frac{1}{2q_{k + 1}^2}$. Thus we have:
      \begin{gather*}
         \begin{split}
            \bigg|\frac{1}{q_k q_{k + 1}}\bigg| = \bigg| \frac{p_{k + 1}}{q_{k + 1}} - \frac{p_k}{q_k}  \bigg|  &= \bigg|(\frac{p_{k + 1}}{q_{k + 1}} - \alpha) + (\alpha - \frac{p_k}{q_k})\bigg|\\
            & = \bigg|\frac{p_{k + 1}}{q_{k + 1}} - \alpha \bigg| + \bigg|\alpha - \frac{p_k}{q_k}\bigg| \\
            & \ge \frac{1}{2q_k^2} + \frac{1}{2q_{k + 1}^2} \\
         \end{split} \\
         \implies 0 \ge \frac{1}{2} (\frac{1}{q_k} - \frac{1}{q_{k + 1}})^2
      \end{gather*}
      Which means that $q_k = q_{k + 1}$, which is a contradiction, thus one of the inequalities must be true.
\end{enumerate}